src/Lean/Elab/Tactic/Do/Internal/VCGen/Driver.lean
@@ -106,6 +106,7 @@ public def work (scope : Scope) (goal : Grind.Goal) : VCGenM Unit := do
   let mut worklist : Array WorkItem := #[{ goal := { goal with mvarId }, scope }]
   while let some s := worklist.back? do
     worklist := worklist.pop
+    if ← s.goal.mvarId.isAssigned then continue
     let goal ← processHypotheses s.goal
     if goal.inconsistent then continue
     match ← solve s.scope goal.mvarId with
